formalization/Fofu_Impl_Base.thy
@@ -4,10 +4,11 @@ imports
   "cava/Libs/Refine_Imperative_HOL/Sepref"
   "cava/Libs/Refine_Imperative_HOL/Heaps/Array_List"
   "~~/src/HOL/Library/Rewrite"
+  Refine_Monadic_Syntax_Sugar
 begin
   hide_type (open) List_Seg.node
 
-
+  interpretation Refine_Monadic_Syntax .
 
 
 end
